\documentclass[]{article}
\usepackage[margin=0.8in]{geometry}

%opening
\title{Stochastic survival of the densest in neurons}
\author{}

\begin{document}
\maketitle
	

\section{Glossary}
	
	\noindent \textbf{variables:} \\
	$W_s$ = number of wildtype mtDNA molecules in the soma \\
	$M_s$ = number of mutant mtDNA molecules in the soma \\
	$W_a$ = number of wildtype mtDNA molecules in the axon \\
	$M_a$ = number of mutant mtDNA molecules in the axon \\
	
	\noindent \textbf{parameters:} \\
	$\mu$ = death rate or degradation rate \\
	$\gamma$ = transport rate between two units \\
	$\delta_m$ = mutant deficiency ratio \\
	$C_b$ = adaptive birth rate control strength parameter \\
	$C_t$ = adaptive transport rate control strength parameter \\
	$NSS_A$ = carrying capacity of axon \\
	$NSS_S$ = carrying capacity of soma \\
	
\pagebreak	
\section{Equations governing per capita reaction rates and rates of change in the model}
	
	\subsection{Per capita rates:}
	
	All per capita reaction rates are identical for wildtype (wt) and mutant (mt) mtDNA molecules, and defined as follows:

	\subsubsection{Birth rates:}
	
	mtDNA is produced in the soma only. The rate of production is sufficient to supply both the soma and the axon.

	\begin{equation}
		Birth_{soma} = 2\mu + C_b \times (Nss_{S}-W_s-\delta_m M_s) 
	\end{equation}
	
	\begin{equation}
		Birth_{axon} = 0
	\end{equation}
	
	\subsubsection{Death rates:}
	
	mtDNA is degraded with equal rates in the soma and axon. 
	
	\begin{equation}
		Death_{soma} = \mu
	\end{equation}
	
	\begin{equation}
		Death_{axon} = \mu
	\end{equation}
	
	\subsubsection{Transport rates:}
	
	mtDNA is transported between the soma and the axon. At steady state, anterograde (soma to axon) transport is 2x the rate of retrograde transport. 
	
	\begin{equation}
		Move_{soma-axon} = 2\gamma + C_t \times (Nss_{A}-W_a-\delta_m M_a) 
	\end{equation}
	
	\begin{equation}
		Move_{axon-soma} = \gamma
	\end{equation}
	
	\subsection{Absolute rates of change:}

	Thus the absolute rates of change for the four model variables are:

	\begin{equation}
		\frac{d W_s}{d t} = W_s \times \left( [2\mu + C_b \times (Nss_{S}-W_s-\delta_m M_s) ] - [\mu] - [2\gamma + C_t \times (Nss_A - W_a - \delta_m M_a)]\right) + W_a \times [\gamma] 
	\end{equation}
	
	\begin{equation}
		\frac{d M_s}{d t} = M_s \times \left( [2\mu + C_b \times (Nss_{S}-W_s-\delta_m M_s) ] - [\mu] - [2\gamma + C_t \times (Nss_A - W_a - \delta_m M_a)]\right) + M_a \times [\gamma] 
	\end{equation}
	
	\begin{equation}
		\frac{d W_a}{d t} = W_a \times \left( [0] - [\mu] - [\gamma] \right) + W_s \times [2\gamma + C_t \times (Nss_A - W_a - \delta_m M_a)]
	\end{equation}
	
	\begin{equation}
		\frac{d M_a}{d t} = M_a \times \left( [0] - [\mu] - [\gamma] \right) + M_s \times [2\gamma + C_t \times (Nss_A - W_a - \delta_m M_a)]
	\end{equation}

\section{Steady states and simplification}
	
	A crucial steady state for the system occurs when both the soma and the axon are at carrying capacity, and the ratio of wild-type to mutant molecules, and the absolute number of molecules is identical in both units:
	
	\begin{equation}
		W_s = W_a \land M_s = M_a \land Nss_{S} = Nss_{A} \land Nss_{S}-W_s-\delta_m M_s = 0 \land Nss_{A}-W_a-\delta_m M_a = 0
	\end{equation}
	
	In such cases, the adaptive birth rate and transport rate terms are both 0:
	
	\begin{equation}
		C_b \times (Nss_{S}-W_s-\delta_m M_s) = 0 \land C_t \times (Nss_{A}-W_a-\delta_m M_a) = 0
	\end{equation}
	
	
	Thus, the system is reduced such that the rates are:
	
		\begin{equation}
		Birth_{soma} = 2\mu
	\end{equation}
	
	\begin{equation}
		Birth_{axon} = 0
	\end{equation}
	
	\begin{equation}
		Death_{soma} = \mu
	\end{equation}
	
	\begin{equation}
		Death_{axon} = \mu
	\end{equation}
		
	\begin{equation}
		Move_{soma-axon} = 2\gamma
	\end{equation}
	
	\begin{equation}
		Move_{axon-soma} = \gamma
	\end{equation}

	Thus the absolute rates of change for the four model variables are:
	
	\begin{equation}
		\frac{d W_s}{d t} = W_s \times [ 2\mu -\mu - 2\gamma] + W_a \times [\gamma] = 0
	\end{equation}

	\begin{equation}
		\frac{kd M_s}{d t} = M_s \times [ 2\mu -\mu - 2\gamma] + M_a \times [\gamma] = 0
	\end{equation}

	\begin{equation}
		\frac{dl W_a}{d t} = W_a \times [- \mu - \gamma ] + W_s \times [2\gamma] = 0
	\end{equation}
	
	\begin{equation}
		\frac{d M_a}{d t} = M_a \times [- \mu - \gamma ] + M_s \times [2\gamma] = 0
	\end{equation}
	
	Thus $\mu = \gamma$.
	


\section{simplified model}

\subsection{glossary}

\noindent \textbf{variables:} \\
$W_s$ = number of wildtype mtDNA molecules in the soma \\
$M_s$ = number of mutant mtDNA molecules in the soma \\
$W_a$ = number of wildtype mtDNA molecules in the axon \\
$M_a$ = number of mutant mtDNA molecules in the axon \\

\noindent \textbf{parameters:} \\
$\lambda$ = death/degradation rate and transport rate (replacing $\mu$ and $\gamma$)\\
$\delta_m$ = mutant deficiency ratio \\
$C_b$ = adaptive birth rate control strength parameter \\
$C_t$ = adaptive transport rate control strength parameter \\
$NSS$ = carrying capacity of axon and carrying capacity of soma \\


\subsection{equations with explicit birth, death and transport rates}

\begin{equation}
	\frac{d W_s}{d t} = W_s \times \left( [2\lambda + C_b \times (Nss-W_s-\delta_m M_s) ] - [\lambda] - [2\lambda + C_t \times (Nss - W_a - \delta_m M_a)]\right) + W_a \times [\lambda] 
\end{equation}

\begin{equation}
	\frac{d M_s}{d t} = M_s \times \left( [2\lambda + C_b \times (Nss-W_s-\delta_m M_s) ] - [\lambda] - [2\lambda + C_t \times (Nss - W_a - \delta_m M_a)]\right) + M_a \times [\lambda] 
\end{equation}

\begin{equation}
	\frac{d W_a}{d t} = W_a \times \left( [0] - [\lambda] - [\lambda] \right) + W_s \times [2\lambda + C_t \times (Nss - W_a - \delta_m M_a)]
\end{equation}

\begin{equation}
	\frac{d M_a}{d t} = M_a \times \left( [0] - [\lambda] - [\lambda] \right) + M_s \times [2\lambda + C_t \times (Nss - W_a - \delta_m M_a)]
\end{equation}		
\pagebreak
\subsection{new eqs.}

\begin{equation}
	\frac{d W_s}{d t} = W_s \times \left( [2\mu + C_b \times (Nss-W_s-\delta_m M_s) ] - [\mu] - [2\gamma]\right) + W_a \times [\gamma] 
\end{equation}

\begin{equation}
	\frac{d M_s}{d t} = M_s \times \left( [2\mu + C_b \times (Nss-W_s-\delta_m M_s) ] - [\mu] - [2\gamma]\right) + M_a \times [\gamma] 
\end{equation}

\begin{equation}
	\frac{d W_a}{d t} = W_a \times \left( [0] - [\mu] - [\gamma] \right) + W_s \times [2\gamma]
\end{equation}

\begin{equation}
	\frac{d M_a}{d t} = M_a \times \left( [0] - [\mu] - [\gamma] \right) + M_s \times [2\gamma]
\end{equation}		

\end{document}
